Unify register and stack cases in Locmap.set
Locmap.set now uniformly uses `Val.load_result` to model stores to registers
and to stack slots equivalently.

backend/Locations.v
@@ -331,33 +331,25 @@ Module Locmap.
   Definition set (l: loc) (v: val) (m: t) : t :=
     fun (p: loc) =>
       if Loc.eq l p then
-        match l with
-        | R r => if Val.has_type_dec v (mreg_type r) then v else Vundef
-        | S sl ofs ty => Val.load_result (chunk_of_type ty) v
-        end
+        Val.load_result (chunk_of_type (Loc.type l)) v
       else if Loc.diff_dec l p then
         m p
       else Vundef.
 
   Lemma gss: forall l v m,
-    (set l v m) l =
-    match l with
-    | R r => if Val.has_type_dec v (mreg_type r) then v else Vundef
-    | S sl ofs ty => Val.load_result (chunk_of_type ty) v
-    end.
+    (set l v m) l = Val.load_result (chunk_of_type (Loc.type l)) v.
   Proof.
     intros. unfold set. apply dec_eq_true.
   Qed.
 
   Lemma gss_reg: forall r v m, Val.has_type v (mreg_type r) -> (set (R r) v m) (R r) = v.
   Proof.
-    intros. unfold set. rewrite dec_eq_true, pred_dec_true; auto.
+    intros. unfold set. rewrite dec_eq_true, Val.load_result_same; auto.
   Qed.
 
   Lemma gss_typed: forall l v m, Val.has_type v (Loc.type l) -> (set l v m) l = v.
   Proof.
-    intros. rewrite gss. destruct l.
-    rewrite pred_dec_true; auto. apply Val.load_result_same; auto.
+    intros. rewrite gss. apply Val.load_result_same; auto.
   Qed.
 
   Lemma gso: forall l v m p, Loc.diff l p -> (set l v m) p = m p.
@@ -384,10 +376,10 @@ Module Locmap.
   Lemma gus: forall ll l m, In l ll -> (undef ll m) l = Vundef.
   Proof.
     assert (P: forall ll l m, m l = Vundef -> (undef ll m) l = Vundef).
-      induction ll; simpl; intros. auto. apply IHll.
+    { induction ll; simpl; intros. auto. apply IHll.
       unfold set. destruct (Loc.eq a l).
-      destruct a. auto. destruct ty; reflexivity.
-      destruct (Loc.diff_dec a l); auto.
+      apply Val.load_result_same; auto. simpl; auto.
+      destruct (Loc.diff_dec a l); auto. }
     induction ll; simpl; intros. contradiction.
     destruct H. apply P. subst a. apply gss_typed. exact I.
     auto.
